left save and restore 2

coqimp/framework/soundness/inssound.v
@@ -1352,6 +1352,1458 @@ Proof.
   simpl in H.
   simpljoin1; eauto.
 Qed.
+
+Definition dom_eq (M m : Memory) :=
+  (forall l, indom l M -> indom l m) /\ (forall l, indom l m -> indom l M).
+
+Lemma frame_asrt_upd :
+  forall M R D id id' F F',
+    (M, (R, F), D) |= {| id, F |} ->
+    exists m, (m, (R, F'), D) |= {| id', F' |} /\ dom_eq M m.
+Proof.
+  intros.
+  simpls.
+  simpljoin1.
+  unfolds regSt.
+  simpljoin1.
+  simpls.
+  exists (MemMap.set (R cwp) (Some id') emp).
+  repeat (split; eauto).
+  {
+    subst.
+    intros.
+    clear - H.
+    unfolds indom.
+    simpljoin1.
+    unfolds MemMap.set.
+    destruct_addreq_H.
+  }
+  {
+    subst.
+    intros.
+    clear - H.
+    unfolds indom.
+    simpljoin1.
+    unfolds MemMap.set.
+    destruct_addreq_H.
+  }
+Qed.
+
+Ltac sep_star_split_tac :=
+  match goal with
+  | H : _ |= ?p1 ** ?p2 |- _ =>
+    let x := fresh in
+    let x1 := fresh in
+    eapply sep_star_split in H;
+    destruct H as [ x [x1 H] ]; simpljoin1;
+    destruct_state x; destruct_state x1;
+    sep_star_split_tac
+  | _ => idtac
+  end.
+
+Lemma disj_sep_star_merge :
+  forall m1 m2 R F D p1 p2,
+    (m1, (R, F), D) |= p1 ->
+    (m2, (R, F), D) |= p2 ->
+    disjoint m1 m2 ->
+    (merge m1 m2, (R, F), D) |= p1 ** p2.
+Proof.
+  intros.
+  simpl.
+  exists (m1, (R, F), D) (m2, (R, F), D).
+  repeat (split; eauto).
+Qed.
+
+Lemma disj_dom_eq_still :
+  forall m1 m2 m1' m2',
+    disjoint m1 m2 ->
+    dom_eq m1 m1' -> dom_eq m2 m2' ->
+    disjoint m1' m2'.
+Proof.
+  intros.
+  unfolds disjoint.
+  intros.
+  specialize (H x).
+  destruct (m1 x) eqn:Heqe1.
+  {
+    destruct (m1' x) eqn:Heqe1';
+      destruct (m2 x) eqn:Heqe2;
+      destruct (m2' x) eqn:Heqe2'; eauto.
+    clear - Heqe2 H1 Heqe2'.
+    unfolds dom_eq.
+    simpljoin1.
+    assert (indom x m2').
+    unfold indom; eauto.
+    eapply H0 in H1; eauto.
+    unfolds indom.
+    simpljoin1.
+    tryfalse.
+  }
+  {
+    destruct (m1' x) eqn:Heqe1';
+      destruct (m2 x) eqn:Heqe2;
+      destruct (m2' x) eqn:Heqe2'; eauto.
+    clear - Heqe1 Heqe1' H0.
+    unfolds dom_eq.
+    simpljoin1.
+    assert (indom x m1').
+    unfold indom; eauto.
+    eapply H0 in H1; eauto.
+    unfolds indom.
+    simpljoin1.
+    tryfalse.
+    clear - Heqe1 H0 Heqe1'.
+    unfolds dom_eq.
+    simpljoin1.
+    assert (indom x m1').
+    unfold indom; eauto.
+    eapply H0 in H1.
+    unfolds indom.
+    simpljoin1.
+    tryfalse.
+  }
+Qed.
+
+Lemma dom_eq_emp :
+  dom_eq emp emp.
+Proof.
+  unfolds dom_eq.
+  split; intros; eauto.
+Qed.
+
+Lemma dom_eq_memset_same_addr_stable :
+  forall m1 m2 l v v',
+    dom_eq m1 m2 ->
+    dom_eq (MemMap.set l (Some v) m1) (MemMap.set l (Some v') m2).
+Proof.
+  intros.
+  unfolds dom_eq.
+  simpljoin1.
+  split.
+  {
+    clear - H.
+    intros.
+    unfold indom in H0.
+    simpljoin1.
+    unfolds MemMap.set.
+    destruct_addreq_H.
+    {
+      subst.
+      inversion H0; subst.
+      unfold indom.
+      exists v'.
+      destruct_addreq.
+    }
+    {
+      unfold indom.
+      assert (indom l0 m1).
+      unfolds indom; eauto.
+      eapply H in H2.
+      unfolds indom.
+      simpljoin1.
+      destruct_addreq.
+    }
+  }
+  {
+    intros.
+    unfold indom in H1.
+    simpljoin1.
+    unfolds MemMap.set.
+    destruct_addreq_H.
+    {
+      inversion H1; subst.
+      unfold indom.
+      exists v.
+      destruct_addreq.
+    }
+    {
+      assert (indom l0 m2).
+      unfold indom; eauto.
+      eapply H0 in H3.
+      unfolds indom.
+      simpljoin1.
+      exists x0.
+      destruct_addreq.
+    }
+  }
+Qed.
+
+Lemma disj_merge_disj_sep :
+  forall m1 m2 m3,
+    disjoint m1 (merge m2 m3) ->
+    disjoint m1 m2 /\ disjoint m1 m3.
+Proof.
+  intros.
+  split.
+  eapply disj_merge_disj_sep1; eauto.
+  eapply disj_merge_disj_sep2; eauto.
+Qed.
+
+Lemma dom_eq_merge_some_addr_stable :
+  forall m1 m2 l w w',
+    dom_eq m1 m2 ->
+    dom_eq (merge (MemMap.set l (Some w) emp) m1)
+           (merge (MemMap.set l (Some w') emp) m2).
+Proof.
+  intros.
+  unfolds dom_eq.
+  simpljoin1.
+  split.
+  {
+    intros.
+    unfold indom in H1.
+    simpljoin1.
+    unfolds merge.
+    unfold indom.
+    unfolds MemMap.set.
+    destruct_addreq.
+    {
+      simpl in H1.
+      simpl.
+      assert (indom l0 m1).
+      unfold indom; eauto.
+      eapply H in H3.
+      unfolds indom; eauto.
+    }
+  }
+  {
+    intros.
+    unfold indom in H1.
+    simpljoin1.
+    unfolds merge.
+    unfolds MemMap.set.
+    destruct_addreq_H.
+    inversion H1; subst.
+    unfold indom.
+    destruct_addreq.
+    unfold indom.
+    destruct_addreq.
+    simpls.
+    assert (indom l0 m2).
+    {
+      unfold indom; eauto.
+    }
+    eapply H0 in H4.
+    unfolds indom; eauto.
+  }
+Qed.
+  
+Ltac disj_reg_solve :=
+  match goal with
+  | H : disjoint (MemMap.set ?l1 (Some ?v1) emp)
+                 (merge (MemMap.set ?l2 (Some ?v2) emp) ?m) |-
+    disjoint (MemMap.set ?l1 (Some ?v1') emp)
+             (merge (MemMap.set ?l2 (Some ?v2') emp) ?m') =>
+    eapply disj_merge_disj_sep in H;
+    let H1 := fresh in
+    let H2 := fresh in
+    destruct H as [H1 H2];
+    eapply disj_sep_merge_still;
+    [
+      eapply MemSet_same_addr_disj_stable;
+      eapply MemSet_same_addr_disj_stable2; eauto |
+      disj_reg_solve
+    ]
+  | _ =>
+    try (eapply MemSet_same_addr_disj_stable;
+         eapply MemSet_same_addr_disj_stable2; eauto)
+  end.
+  
+Lemma reg_frame_upd :
+  forall (rr0 rr1 rr2 rr3 rr4 rr5 rr6 rr7 : GenReg)
+    w0 w1 w2 w3 w4 w5 w6 w7 w0' w1' w2' w3' w4' w5' w6' w7' 
+    M R F F' D,
+    (M, (R, F), D) |=
+                   rr0 |=> w0 **
+                   rr1 |=> w1 **
+                   rr2 |=> w2 ** rr3 |=> w3 ** rr4 |=> w4 **
+                   rr5 |=> w5 ** rr6 |=> w6 ** rr7 |=> w7 ->
+  exists m,
+    (m, (R, F'), D) |=
+                   rr0 |=> w0' **
+                   rr1 |=> w1' **
+                   rr2 |=> w2' ** rr3 |=> w3' ** rr4 |=> w4' **
+                   rr5 |=> w5' ** rr6 |=> w6' ** rr7 |=> w7' /\ dom_eq M m.
+Proof.
+  intros.
+  sep_star_split_tac.
+  simpl in H3, H2, H5, H7, H9, H11, H13.
+  simpljoin1.
+
+  simpl in H, H0, H1, H4, H6, H8, H10, H12.
+  unfolds regSt.
+  simpl in H, H0, H1, H4, H6, H8, H10, H12.
+  simpljoin1.
+  rename r12 into R.
+
+  exists
+    (merge (MemMap.set (R rr0) (Some w0') emp)
+    (merge (MemMap.set (R rr1) (Some w1') emp)
+           (merge (MemMap.set (R rr2) (Some w2') emp)
+                  (merge (MemMap.set (R rr3) (Some w3') emp)
+                         (merge (MemMap.set (R rr4) (Some w4') emp)
+                                (merge (MemMap.set (R rr5) (Some w5') emp)
+                                       (merge (MemMap.set (R rr6) (Some w6') emp)
+                                              (MemMap.set (R rr7) (Some w7') emp)))))))).
+  split.
+ 
+  eapply disj_sep_star_merge; eauto.
+  simpl. unfold regSt.
+  simpl; eauto.
+
+  eapply disj_sep_star_merge; eauto.
+  simpl; unfold regSt.
+  simpl; eauto.
+
+  eapply disj_sep_star_merge; eauto.
+  simpl; unfold regSt.
+  simpl; eauto.
+
+  eapply disj_sep_star_merge; eauto.
+  simpl; unfold regSt.
+  simpl; eauto.
+
+  eapply disj_sep_star_merge; eauto.
+  simpl; unfold regSt.
+  simpl; eauto.
+
+  eapply disj_sep_star_merge; eauto.
+  simpl; unfold regSt.
+  simpl; eauto.
+
+  eapply disj_sep_star_merge; eauto.
+  simpl; unfold regSt.
+  simpl; eauto.
+  
+  simpl; unfold regSt.
+  simpl; eauto.
+
+  disj_reg_solve.
+  disj_reg_solve.
+  disj_reg_solve.
+  disj_reg_solve.
+  disj_reg_solve.
+  disj_reg_solve.
+  disj_reg_solve.
+
+  repeat (eapply dom_eq_merge_some_addr_stable; eauto).
+  eapply dom_eq_memset_same_addr_stable.
+  eapply dom_eq_emp.
+Qed.
+  
+Lemma OutRegs_asrt_upd :
+  forall M R F F' D fm fm',
+    (M, (R, F), D) |= OutRegs fm ->
+    exists m, (m, (R, F'), D) |= OutRegs fm' /\ dom_eq M m.
+Proof.
+  intros.
+  unfolds OutRegs.
+  destruct fm, fm'.
+  eapply reg_frame_upd; eauto.
+Qed.
+
+Lemma LocalRegs_asrt_upd :
+  forall M R F F' D fm fm',
+    (M, (R, F), D) |= LocalRegs fm ->
+    exists m, (m, (R, F'), D) |= LocalRegs fm' /\ dom_eq M m.
+Proof.
+  intros.
+  unfolds LocalRegs.
+  destruct fm, fm'.
+  eapply reg_frame_upd; eauto.
+Qed.
+
+Lemma InRegs_asrt_upd :
+  forall M R F F' D fm fm',
+    (M, (R, F), D) |= InRegs fm ->
+    exists m, (m, (R, F'), D) |= InRegs fm' /\ dom_eq M m.
+Proof.
+  intros.
+  unfolds InRegs.
+  destruct fm, fm'.
+  eapply reg_frame_upd; eauto.
+Qed.
+
+Lemma dom_eq_merge_still :
+  forall m1 m1' m2 m2',
+    dom_eq m1 m1' -> dom_eq m2 m2' ->
+    dom_eq (merge m1 m2) (merge m1' m2').
+Proof.
+  intros.
+  unfolds dom_eq.
+  split.
+  {
+    intros.
+    simpljoin1.
+    unfold indom in H1.
+    simpljoin1.
+    unfolds merge.
+    destruct (m1 l) eqn:Heqe.
+    {
+      inversion H1; subst.
+      assert (indom l m1).
+      unfold indom; eauto.
+      eapply H in H4.
+      unfolds indom; simpljoin1.
+      eexists.
+      rewrite H4; eauto.
+    }
+    {
+      unfold indom.
+      destruct (m1' l) eqn:Heqe'.
+      assert (indom l m1').
+      unfold indom; eauto.
+      eapply H3 in H4.
+      unfolds indom.
+      simpljoin1.
+      rewrite Heqe in H4. tryfalse.
+      assert (indom l m2).
+      unfold indom; eauto.
+      eapply H0 in H4; eauto.
+    }
+  }
+  {
+    intros.
+    unfold indom in H1.
+    simpljoin1.
+    unfolds merge.
+    destruct (m1' l) eqn:Heqe.
+    {
+      inversion H1; subst.
+      assert (indom l m1').
+      {
+        unfold indom; eauto.
+      }
+      eapply H3 in H4.
+      unfolds indom.
+      simpljoin1.
+      rewrite H4; eauto.
+    }
+    {
+      unfold indom.
+      destruct (m1 l) eqn:Heqe1.
+      {
+        assert (indom l m1).
+        unfold indom; eauto.
+        eapply H in H4.
+        unfolds indom; simpljoin1.
+        rewrite Heqe in H4.
+        tryfalse.
+      }
+      {
+        assert (indom l m2').
+        unfold indom; eauto.
+        eapply H2 in H4; eauto.
+      }
+    }
+  }
+Qed.
+  
+Lemma Regs_asrt_upd :
+  forall M R F F' D fm1 fm1' fm2 fm2' fm3 fm3',
+    (M, (R, F), D) |= Regs fm1 fm2 fm3 ->
+    exists m, (m, (R, F'), D) |= Regs fm1' fm2' fm3' /\ dom_eq M m.
+Proof.
+  intros.
+  unfolds Regs.
+  eapply sep_star_split in H.
+  simpljoin1.
+  destruct_state x.
+  destruct_state x0.
+  eapply sep_star_split in H0.
+  simpljoin1.
+  destruct_state x.
+  destruct_state x0.
+  eapply OutRegs_asrt_upd with (F' := F') (fm' := fm1') in H.
+  eapply LocalRegs_asrt_upd with (F' := F') (fm' := fm2') in H0.
+  eapply InRegs_asrt_upd with (F' := F') (fm' := fm3') in H2.
+  simpljoin1.
+  renames x1 to m0', x0 to m1', x to m2'.
+  simpl in H3, H1.
+  simpljoin1.
+  rename r2 into R.
+  exists (merge m0' (merge m1' m2')).
+  split.
+  {
+    eapply disj_sep_star_merge; eauto.
+    eapply disj_sep_star_merge; eauto.
+    eapply disj_dom_eq_still.
+    eapply H3.
+    eauto.
+    eauto.
+    eapply disj_dom_eq_still; eauto.
+    eapply dom_eq_merge_still; eauto.
+  }
+  {
+    eapply dom_eq_merge_still; eauto.
+    eapply dom_eq_merge_still; eauto.
+  }
+Qed.
+
+Lemma regdlySt_changeFrm_stable :
+  forall n s w M R F F' D,
+    regdlySt n s w (M, (R, F), D) ->
+    regdlySt n s w (M, (R, F'), D).
+Proof.
+  intro n.
+  induction n; intros.
+  -
+    unfolds regdlySt; eauto.
+  -
+    simpls.
+    destruct H; eauto.
+Qed.
+
+Lemma asrt_FrmFree_changefrm_stable :
+  forall p M R F F' D,
+    (M, (R, F), D) |= p -> ~ indom (R cwp) M ->
+    (M, (R, F'), D) |= p.
+Proof.
+  intros p.
+  induction p; intros; simpl; eauto; tryfalse.
+
+  -
+    simpl in H.
+    simpljoin1.
+    exists x.
+    repeat (split; eauto).
+    destruct H1.
+    left.
+    eapply regdlySt_changeFrm_stable; eauto.
+    eauto.
+
+  - 
+    simpl in H.
+    simpljoin1.
+    unfolds regSt.
+    simpls.
+    simpljoin1.
+    false.
+    eapply H0.
+    unfold indom.
+    unfold MemMap.set.
+    destruct_addreq.
+
+  - 
+    simpl in H0.
+    simpljoin1.
+    simpl in H. 
+    destruct H.
+    eauto.
+    
+  - 
+    simpl in H.
+    destruct H.
+    eauto.
+    eauto.
+
+  -
+    simpl in H.
+    simpljoin1.
+    destruct_state x.
+    destruct_state x0.
+    simpls.
+    simpljoin1.
+    exists (m, (r0, F'), d0) (m0, (r0, F'), d0).
+    simpl.
+    repeat (split; eauto).
+    eapply IHp1; eauto.
+    intro.
+    eapply H0.
+    eapply indom_merge_still; eauto.
+    eapply IHp2; eauto.
+    intro.
+    eapply H0.
+    eapply indom_merge_still2; eauto.
+    
+  -
+    simpljoin1; eauto.
+    simpl in H0.
+    simpljoin1; eauto.
+Qed.
+
+Lemma same_m_dom_eq:
+  forall m,
+    dom_eq m m.
+Proof.
+  unfold dom_eq.
+  intros.
+  split; intros; eauto.
+Qed.
+
+Lemma indom_dom_eq_merge_subst :
+  forall l m1 m1' m2,
+    indom l (merge m1 m2) ->
+    dom_eq m1 m1' ->
+    indom l (merge m1' m2).
+Proof.
+  intros.
+  unfolds indom.
+  unfolds dom_eq.
+  simpljoin1.
+  unfolds merge.
+  destruct (m1 l) eqn:Heqe1.
+  {
+    assert (indom l m1).
+    unfold indom; eauto.
+    eapply H0 in H2; eauto.
+    unfolds indom.
+    simpljoin1; eauto.
+    eexists.
+    rewrite H2; eauto.
+  }
+  {
+    destruct (m1' l) eqn:Heqe2; eauto.
+  }
+Qed.
+
+Lemma indom_dom_eq_merge_subst2 :
+  forall l m1 m2 m2',
+    indom l (merge m1 m2) ->
+    dom_eq m2 m2' ->
+    indom l (merge m1 m2').
+Proof.
+  intros.
+  unfolds indom.
+  unfolds dom_eq.
+  simpljoin1.
+  unfolds merge. 
+  destruct (m1 l) eqn:Heqe1.
+  {
+    inversion H; eauto.
+  }
+  {
+    assert (indom l m2).
+    unfold indom; eauto.
+    eapply H0 in H2; eauto.
+  }
+Qed.
+  
+Lemma dom_eq_merge_subst1 :
+  forall m m' m1 m2,
+    dom_eq m m' ->
+    dom_eq (merge m m1) m2 ->
+    dom_eq (merge m' m1) m2.
+Proof.
+  intros.
+  unfolds dom_eq.
+  split.
+  {
+    intros.
+    simpljoin1.
+    eapply H0.
+    eapply indom_dom_eq_merge_subst; eauto.
+    unfold dom_eq; eauto.
+  }
+  {
+    simpljoin1.
+    intros.
+    eapply H1 in H3.
+    eapply indom_dom_eq_merge_subst; eauto.
+    unfold dom_eq; eauto.
+  }
+Qed.
+
+Lemma dom_eq_sym :
+  forall m m',
+    dom_eq m m' -> dom_eq m' m.
+Proof.
+  intros.
+  unfolds dom_eq.
+  simpljoin1.
+  split.
+  {
+    intros; eauto.
+  }
+  {
+    intros; eauto.
+  }
+Qed.
+
+Lemma dom_eq_trans :
+  forall m1 m2 m3,
+    dom_eq m1 m2 -> dom_eq m2 m3 ->
+    dom_eq m1 m3.
+Proof.
+  intros.
+  unfolds dom_eq.
+  simpljoin1.
+  split.
+  {
+    intros.
+    eapply H in H3.
+    eauto.
+  }
+  {
+    intros.
+    eapply H1 in H3; eauto.
+  }
+Qed.
+
+Lemma disj_in_m1_merge_still :
+  forall m1 m2 l v,
+    disjoint m1 m2 -> m1 l = Some v ->
+    merge m1 m2 l = Some v.
+Proof.
+  intros.
+  unfold merge.
+  rewrite H0; eauto.
+Qed.
+
+Lemma disj_in_m2_merge_still :
+  forall m1 m2 l v,
+    disjoint m1 m2 -> m2 l = Some v ->
+    merge m1 m2 l = Some v.
+Proof.
+  intros.
+  unfold merge.
+  destruct (m1 l) eqn:Heqe.
+  {
+    unfolds disjoint.
+    specialize (H l).
+    rewrite Heqe in H.
+    rewrite H0 in H; tryfalse.
+  }
+  {
+    eauto.
+  }
+Qed.
+
+Ltac fetch_frame_merge_solve1 :=
+  match goal with
+  | H : context [?m (?R ?rr)] |- _ =>
+    let Heqe := fresh in
+    destruct (m (R rr)) eqn:Heqe;
+    [eapply disj_in_m1_merge_still in Heqe;
+     [rewrite Heqe; simpl; fetch_frame_merge_solve1 | eauto]
+    | tryfalse]
+  | _ => idtac
+  end.
+
+Ltac fetch_frame_merge_solve2 :=
+  match goal with
+  | H : context [?m (?R ?rr)] |- _ =>
+    let Heqe := fresh in
+    destruct (m (R rr)) eqn:Heqe;
+    [eapply disj_in_m2_merge_still in Heqe;
+     [rewrite Heqe; simpl; fetch_frame_merge_solve2 | eauto]
+    | tryfalse]
+  | _ => idtac
+  end.
+
+Lemma fetch_frm_disj_merge_still1 :
+  forall m m1 R rr0 rr1 rr2 rr3 rr4 rr5 rr6 rr7 fm,
+    fetch_frame m R rr0 rr1 rr2 rr3 rr4 rr5 rr6 rr7 = Some fm ->
+    disjoint m m1 ->
+    fetch_frame (merge m m1) R rr0 rr1 rr2 rr3 rr4 rr5 rr6 rr7 = Some fm.
+Proof.
+  intros.
+  unfolds fetch_frame, eval_reg.
+  fetch_frame_merge_solve1.
+  inversion H.
+  eauto.
+Qed.
+
+Lemma fetch_frm_disj_merge_still2 :
+  forall m m1 R rr0 rr1 rr2 rr3 rr4 rr5 rr6 rr7 fm,
+    fetch_frame m R rr0 rr1 rr2 rr3 rr4 rr5 rr6 rr7 = Some fm ->
+    disjoint m1 m ->
+    fetch_frame (merge m1 m) R rr0 rr1 rr2 rr3 rr4 rr5 rr6 rr7 = Some fm.
+Proof.
+  intros.
+  unfolds fetch_frame, eval_reg.
+  fetch_frame_merge_solve2.
+  inversion H.
+  eauto.
+Qed.
+
+Lemma fetch_disj_merge_still1 :
+  forall m R fms m1,
+    fetch m R = Some fms ->
+    disjoint m m1 ->
+    fetch (merge m m1) R = Some fms.
+Proof.
+  intros.
+  unfolds fetch.
+  destruct (fetch_frame m R r8 r9 r10 r11 r12 r13 r14 r15) eqn:Heqe1; tryfalse.
+  eapply fetch_frm_disj_merge_still1 in Heqe1; eauto.
+  rewrite Heqe1. 
+  destruct (fetch_frame m R r16 r17 r18 r19 r20 r21 r22 r23) eqn:Heqe2; tryfalse.
+  eapply fetch_frm_disj_merge_still1 in Heqe2; eauto.
+  rewrite Heqe2.
+  destruct (fetch_frame m R r24 r25 r26 r27 r28 r29 r30 r31) eqn:Heqe3; tryfalse.
+  eapply fetch_frm_disj_merge_still1 in Heqe3; eauto.
+  rewrite Heqe3; eauto.
+Qed.
+  
+Lemma fetch_disj_merge_still2 :
+  forall m R fms m1,
+    fetch m R = Some fms ->
+    disjoint m1 m ->
+    fetch (merge m1 m) R = Some fms.
+Proof.
+  intros.
+  unfolds fetch.
+  destruct (fetch_frame m R r8 r9 r10 r11 r12 r13 r14 r15) eqn:Heqe1; tryfalse.
+  eapply fetch_frm_disj_merge_still2 in Heqe1; eauto.
+  rewrite Heqe1. 
+  destruct (fetch_frame m R r16 r17 r18 r19 r20 r21 r22 r23) eqn:Heqe2; tryfalse.
+  eapply fetch_frm_disj_merge_still2 in Heqe2; eauto.
+  rewrite Heqe2.
+  destruct (fetch_frame m R r24 r25 r26 r27 r28 r29 r30 r31) eqn:Heqe3; tryfalse.
+  eapply fetch_frm_disj_merge_still2 in Heqe3; eauto.
+  rewrite Heqe3; eauto.
+Qed.
+
+Lemma disj_sym :
+  forall m1 m2,
+    disjoint m1 m2 -> disjoint m2 m1.
+Proof.
+  intros.
+  unfolds disjoint.
+  intros.
+  specialize (H x).
+  destruct (m1 x) eqn:Heqe1;
+    destruct (m2 x) eqn:Heqe2; tryfalse; eauto.
+Qed.
+
+Lemma merge_assoc :
+  forall m1 m2 m3,
+    merge m1 (merge m2 m3) = merge (merge m1 m2) m3.
+Proof.
+  intros.
+  unfold merge.
+  eapply functional_extensionality.
+  intros.
+  destruct (m1 x) eqn:Heqe1;
+    destruct (m2 x) eqn:Heqe2;
+    simpl; tryfalse; eauto.
+Qed.
+
+Lemma disj_merge_reverse_eq :
+  forall m1 m2,
+    disjoint m1 m2 ->
+    merge m1 m2 = merge m2 m1.
+Proof.
+  intros.
+  eapply functional_extensionality.
+  intros.
+  unfolds merge.
+  destruct (m1 x) eqn:Heqe1;
+    destruct (m2 x) eqn:Heqe2; simpl; eauto; tryfalse.
+  unfolds disjoint.
+  specialize (H x).
+  rewrite Heqe1 in H;
+    rewrite Heqe2 in H; tryfalse.
+Qed.
+
+Lemma merge_lift :
+  forall m1 m2 m3,
+    disjoint m1 m2 ->
+    merge m1 (merge m2 m3) = merge m2 (merge m1 m3).
+Proof.
+  intros.
+  unfold merge.
+  eapply functional_extensionality; eauto.
+  intros.
+  destruct (m1 x) eqn:Heqe1;
+    destruct (m2 x) eqn:Heqe2; tryfalse; eauto.
+  unfolds disjoint.
+  specialize (H x).
+  rewrite Heqe1 in H;
+    rewrite Heqe2 in H; tryfalse.
+Qed.
+
+Lemma get_vl_merge_still2 :
+  forall M m l v,
+    disjoint M m -> m l = Some v ->
+    merge M m l = Some v.
+Proof.
+  intros.
+  unfolds merge.
+  destruct (M l) eqn:Heqe; tryfalse.
+  unfolds disjoint.
+  specialize (H l).
+  rewrite Heqe in H.
+  rewrite H0 in H.
+  tryfalse.
+  eauto.
+Qed.
+
+Lemma sep_star_assoc :
+  forall s p1 p2 p3,
+    s |= p1 ** p2 ** p3 ->
+    s |= (p1 ** p2) ** p3.
+Proof.
+  intros.
+  destruct_state s.
+  sep_star_split_tac.
+  simpl in H2, H3.
+  simpljoin1.
+  simpl.
+  exists (merge m0 m2, (r3, f3), d3) (m3, (r3, f3), d3).
+  repeat (split; eauto).
+  eapply disj_sym.
+  eapply disj_sep_merge_still; eauto.
+  eapply disj_merge_disj_sep2 in H3.
+  eapply disj_sym; eauto.
+  eapply disj_sym; eauto.
+  rewrite merge_assoc; eauto.
+
+  exists (m0, (r3, f3), d3) (m2, (r3, f3), d3).
+  repeat (split; eauto).
+  eapply disj_merge_disj_sep1 in H3; eauto.
+Qed.
+
+Lemma sep_star_sym :
+  forall s p1 p2,
+    s |= p1 ** p2 ->
+    s |= p2 ** p1.
+Proof.
+  intros.
+  simpls.
+  simpljoin1.
+  exists x0 x.
+  repeat (split; eauto).
+  destruct_state x.
+  destruct_state x0.
+  simpls.
+  simpljoin1.
+  repeat (split; eauto).
+  eapply disj_sym; eauto.
+  rewrite disj_merge_reverse_eq; eauto.
+Qed.
+
+Lemma sep_star_lift :
+  forall s p1 p2 p3,
+    s |= p1 ** p2 ** p3 ->
+    s |= p2 ** p1 ** p3.
+Proof.
+  intros.
+  sep_star_split_tac.
+  simpls; simpljoin1.
+
+  exists (m1, (r2, f2), d2) (merge m m2, (r2, f2), d2).
+  repeat (split; eauto).
+  eapply disj_sep_merge_still; eauto.
+  eapply disj_merge_disj_sep1 in H3.
+  eapply disj_sym; eauto.
+  rewrite merge_lift; eauto.
+  eapply disj_merge_disj_sep1 in H3; eauto.
+
+  exists (m, (r2, f2), d2) (m2, (r2, f2), d2).
+  simpl; eauto.
+  repeat (split; eauto).
+  eapply disj_merge_disj_sep2 in H3; eauto.
+Qed.
+
+Lemma rn_st_v_eval_reg_v :
+  forall M R F D rn w p,
+    (M, (R, F), D) |= rn |=> w ** p ->
+    eval_reg R M rn = Some w.
+Proof.
+  intros.
+  simpls.
+  simpljoin1.
+  destruct_state x.
+  destruct_state x0.
+  simpls.
+  simpljoin1.
+  unfolds regSt.
+  simpls; simpljoin1.
+  unfold eval_reg.
+  unfold merge.
+  unfold MemMap.set.
+  destruct_addreq.
+Qed.
+
+Lemma reg_st_fetch_frame :
+  forall (rr0 rr1 rr2 rr3 rr4 rr5 rr6 rr7 : GenReg) w0 w1 w2 w3 w4 w5 w6 w7
+    M R F D,
+    (M, (R, F), D)
+      |= rr0 |=> w0 **
+      rr1 |=> w1 **
+      rr2 |=> w2 ** rr3 |=> w3 ** rr4 |=> w4 ** rr5 |=> w5 ** rr6 |=> w6 ** rr7 |=> w7 ->
+    fetch_frame M R rr0 rr1 rr2 rr3 rr4 rr5 rr6 rr7 =
+    Some ([[w0, w1, w2, w3, w4, w5, w6, w7]]).
+Proof.
+  intros.
+
+  assert (eval_reg R M rr0 = Some w0).
+  {
+    eapply rn_st_v_eval_reg_v; eauto.
+  }
+  assert (eval_reg R M rr1 = Some w1).
+  {
+    eapply sep_star_lift in H.
+    eapply rn_st_v_eval_reg_v; eauto.
+  }
+  assert (eval_reg R M rr2 = Some w2).
+  {
+    eapply sep_star_assoc in H.
+    eapply sep_star_lift in H.
+    eapply rn_st_v_eval_reg_v; eauto.
+  }
+  assert (eval_reg R M rr3 = Some w3).
+  {
+    do 2 eapply sep_star_assoc in H.
+    eapply sep_star_lift in H.
+    eapply rn_st_v_eval_reg_v; eauto.
+  }
+  assert (eval_reg R M rr4 = Some w4).
+  {
+    do 3 eapply sep_star_assoc in H.
+    eapply sep_star_lift in H.
+    eapply rn_st_v_eval_reg_v; eauto.
+  }
+  assert (eval_reg R M rr5 = Some w5).
+  {
+    do 4 eapply sep_star_assoc in H.
+    eapply sep_star_lift in H.
+    eapply rn_st_v_eval_reg_v; eauto.
+  }
+  assert (eval_reg R M rr6 = Some w6).
+  {
+    do 5 eapply sep_star_assoc in H.
+    eapply sep_star_lift in H.
+    eapply rn_st_v_eval_reg_v; eauto.
+  }
+  assert (eval_reg R M rr7 = Some w7).
+  {
+    do 6 eapply sep_star_assoc in H.
+    eapply sep_star_sym in H.
+    eapply rn_st_v_eval_reg_v in H; eauto.
+  }
+
+  unfold fetch_frame.
+  rewrite H0; eauto.
+  rewrite H1; eauto.
+  rewrite H2; eauto.
+  rewrite H3; eauto.
+  rewrite H4; eauto.
+  rewrite H5; eauto.
+  rewrite H6; eauto.
+  rewrite H7; eauto.
+Qed.
+
+Lemma eval_reg_disj_merge_stable1 :
+  forall m1 m2 R rn v,
+    disjoint m1 m2 ->
+    eval_reg R m1 rn = Some v ->
+    eval_reg R (merge m1 m2) rn = Some v.
+Proof.
+  intros.
+  unfolds eval_reg.
+  unfolds merge.
+  rewrite H0; eauto.
+Qed.
+
+Lemma eval_reg_disj_merge_stable2 :
+  forall m1 m2 R rn v,
+    disjoint m1 m2 ->
+    eval_reg R m2 rn = Some v ->
+    eval_reg R (merge m1 m2) rn = Some v.
+Proof.
+  intros.
+  unfolds eval_reg.
+  unfold merge.
+  destruct (m1 (R rn)) eqn:Heqe; eauto.
+  unfolds disjoint.
+  specialize (H (R rn)).
+  rewrite Heqe in H.
+  rewrite H0 in H; tryfalse.
+Qed.
+
+Lemma eval_opexp_merge_still2 :
+  forall M m R oexp l,
+    eval_opexp R m oexp = Some l -> disjoint M m ->
+    eval_opexp R (merge M m) oexp = Some l.
+Proof.
+  intros.
+  destruct oexp.
+  {
+    simpls.
+    eapply eval_reg_disj_merge_stable2; eauto.
+  }
+  {
+    simpls.
+    eauto.
+  }
+Qed.
+
+Ltac eval_reg_merge_solve1 :=
+  match goal with
+  | H : context [eval_reg ?R ?m ?rn] |- context [eval_reg ?R (merge ?m ?m') ?rn] =>
+    let Heqe := fresh in
+    destruct (eval_reg R m rn) eqn:Heqe;
+    [ eapply eval_reg_disj_merge_stable1 in Heqe; eauto;
+      try rewrite Heqe; eval_reg_merge_solve1 | tryfalse]
+  | _ => idtac
+  end.
+
+Ltac eval_reg_merge_solve2 :=
+  match goal with
+  | H : context [eval_reg ?R ?m ?rn] |- context [eval_reg ?R (merge ?m' ?m) ?rn] =>
+    let Heqe := fresh in
+    destruct (eval_reg R m rn) eqn:Heqe;
+    [ eapply eval_reg_disj_merge_stable2 in Heqe; eauto;
+      try rewrite Heqe; eval_reg_merge_solve2 | tryfalse]
+  | _ => idtac
+  end.
+      
+Lemma fetch_frame_disj_merge_stable1 :
+  forall m1 m2 R rr0 rr1 rr2 rr3 rr4 rr5 rr6 rr7 fm,
+    disjoint m1 m2 ->
+    fetch_frame m1 R rr0 rr1 rr2 rr3 rr4 rr5 rr6 rr7 = Some fm ->
+    fetch_frame (merge m1 m2) R rr0 rr1 rr2 rr3 rr4 rr5 rr6 rr7 = Some fm.
+Proof.
+  intros.
+  unfolds fetch_frame.
+
+  eval_reg_merge_solve1.
+  eauto.
+Qed.
+
+Lemma fetch_frame_disj_merge_stable2 :
+  forall m1 m2 R rr0 rr1 rr2 rr3 rr4 rr5 rr6 rr7 fm,
+    disjoint m1 m2 ->
+    fetch_frame m2 R rr0 rr1 rr2 rr3 rr4 rr5 rr6 rr7 = Some fm ->
+    fetch_frame (merge m1 m2) R rr0 rr1 rr2 rr3 rr4 rr5 rr6 rr7 = Some fm.
+Proof.
+  intros.
+  unfolds fetch_frame.
+
+  eval_reg_merge_solve2.
+  eauto.
+Qed.
+  
+Lemma OutRegs_fetch :
+  forall M R F D fm,
+    (M, (R, F), D) |= OutRegs fm ->
+    fetch_frame M R r8 r9 r10 r11 r12 r13 r14 r15 = Some fm.
+Proof.
+  intros.
+  unfolds OutRegs.
+  destruct fm.
+  eapply reg_st_fetch_frame; eauto.
+Qed.
+
+Lemma LocalRegs_fetch :
+  forall M R F D fm,
+    (M, (R, F), D) |= LocalRegs fm ->
+    fetch_frame M R r16 r17 r18 r19 r20 r21 r22 r23 = Some fm.
+Proof.
+  intros.
+  unfolds LocalRegs.
+  destruct fm.
+  eapply reg_st_fetch_frame; eauto.
+Qed.
+
+Lemma InRegs_fetch :
+  forall M R F D fm,
+    (M, (R, F), D) |= InRegs fm ->
+    fetch_frame M R r24 r25 r26 r27 r28 r29 r30 r31 = Some fm.
+Proof.
+  intros.
+  unfolds InRegs.
+  destruct fm.
+  eapply reg_st_fetch_frame; eauto.
+Qed.
+  
+Lemma Regs_fetch :
+  forall M R F D fm1 fm2 fm3,
+    (M, (R, F), D) |= Regs fm1 fm2 fm3 ->
+    fetch M R = Some [fm1; fm2; fm3].
+Proof.
+  intros.
+  unfolds Regs.
+  eapply sep_star_split in H.
+  simpljoin1.
+  destruct_state x.
+  destruct_state x0.
+  eapply sep_star_split in H0.
+  simpljoin1.
+  destruct_state x.
+  destruct_state x0.
+
+  simpl in H1, H3.
+  simpljoin1.
+
+  eapply OutRegs_fetch in H; eauto.
+  eapply LocalRegs_fetch in H0; eauto.
+  eapply InRegs_fetch in H2; eauto.
+
+  unfold fetch.
+
+  eapply fetch_frame_disj_merge_stable1 with (m2 := merge m1 m2) in H; eauto.
+  rewrite H.
+
+  eapply fetch_frame_disj_merge_stable1 with (m2 := m2) in H0; eauto.
+  eapply fetch_frame_disj_merge_stable2 in H0; eauto.
+  rewrite H0; eauto.
+
+  eapply fetch_frame_disj_merge_stable2 with (m1 := m1) in H2; eauto.
+  eapply fetch_frame_disj_merge_stable2 with (m1 := m) in H2; eauto.
+
+  rewrite H2; eauto.
+Qed.
+
+Lemma indom_setR_merge_eq2 :
+  forall R M rn m v,
+    indom (R rn) m -> disjoint M m ->
+    set_R R (merge M m) rn v = merge M (set_R R m rn v).
+Proof.
+  intros.
+  unfolds set_R. 
+  lets Ht : H. 
+  eapply indom_merge_still with (m := M) in Ht; eauto.
+  rewrite disj_merge_reverse_eq in Ht; eauto.
+  2 : eapply disj_sym; eauto.
+  eapply indom_isindom in H; eauto.
+  eapply indom_isindom in Ht; eauto.
+  rewrite Ht; eauto.
+  rewrite H; eauto.
+  unfolds MemMap.set, merge.
+  eapply functional_extensionality; eauto.
+  intro.
+  destruct (AddrEq.eq x (R rn)) eqn:Heqe1; eauto.
+  subst.
+  destruct (M (R rn)) eqn:Heqe; eauto.
+  clear - H H0 Heqe.
+  unfolds is_indom.
+  destruct (m (R rn)) eqn:Heqe1; eauto.
+  unfolds disjoint.
+  specialize (H0 (R rn)).
+  rewrite Heqe in H0.
+  rewrite Heqe1 in H0.
+  tryfalse.
+  tryfalse.
+Qed.
+
+Lemma disjoint_setR_still2:
+  forall (m1 m2 : Memory) (R : RegFile) (rn : RegName) (v : Word),
+    disjoint m1 m2 ->
+    disjoint m1 (set_R R m2 rn v).
+Proof.
+  intros.
+  unfolds disjoint.
+  intros.
+  specialize (H x).
+  unfold set_R.
+  destruct (m1 x) eqn:Heqe1.
+  {
+    destruct (is_indom (R rn) m2) eqn:Heqe2; tryfalse.
+    {
+      destruct (m2 x) eqn:Heqe3.
+      unfold MemMap.set.
+      destruct_addreq.
+      unfold MemMap.set.
+      destruct_addreq.
+      unfolds is_indom.
+      subst.
+      rewrite Heqe3 in Heqe2; tryfalse.
+      rewrite Heqe3; eauto.
+    }
+    {
+      destruct (m2 x) eqn:Heqe3; tryfalse.
+      eauto.
+    }
+  }
+  {
+    destruct (is_indom (R rn) m2) eqn:Heqe2; tryfalse.
+    {
+      unfolds is_indom.
+      unfolds MemMap.set.
+      destruct_addreq.
+    }
+    {
+      eauto.
+    }
+  }
+Qed.
+  
+Lemma indoms_setRs_merge_eq2 :
+  forall vl M m R,
+    disjoint M m ->
+    indoms (getRs_addr vl R) m ->
+    set_Rs R (merge M m) vl = merge M (set_Rs R m vl).
+Proof.
+  intros vl.
+  induction vl; intros.
+  -
+    simpls.
+    eauto.
+  -
+    destruct a.
+    simpl in H0.
+    simpl.
+    simpljoin1.
+     
+    rewrite indom_setR_merge_eq2; eauto.
+    eapply IHvl.
+    eapply disjoint_setR_still2; eauto.
+    eapply indoms_setR_still; eauto.
+Qed.
+
+Lemma fetch_some_set_frm_merge_eq2 :
+  forall M m (R : RegFile) fm (rr0 rr1 rr2 rr3 rr4 rr5 rr6 rr7 : GenReg),
+    disjoint M m ->
+    indoms [R rr0; R rr1; R rr2; R rr3; R rr4; R rr5; R rr6; R rr7] m ->
+    set_frame R (merge M m) rr0 rr1 rr2 rr3 rr4 rr5 rr6 rr7 fm =
+    merge M (set_frame R m rr0 rr1 rr2 rr3 rr4 rr5 rr6 rr7 fm).
+Proof.
+  intros.
+  unfolds set_frame.
+  destruct fm.
+  eapply indoms_setRs_merge_eq2; eauto.
+Qed.
+
+Lemma dom_eq_setR_stable :
+  forall  M R rn w,
+    dom_eq M (set_R R M rn w).
+Proof.
+  intros.
+  unfolds dom_eq.
+  split.
+  {
+    intros.
+    unfolds set_R.
+    destruct (is_indom (R rn) M) eqn:Heqe.
+    {
+      unfolds MemMap.set.
+      unfolds indom.
+      destruct_addreq.
+    }
+    {
+      eauto.
+    }
+  }
+  {
+    intros.
+    unfolds set_R.
+    destruct (is_indom (R rn) M) eqn:Heqe; eauto.
+    unfolds MemMap.set.
+    unfolds indom.
+    destruct_addreq_H.
+    subst.
+    simpljoin1.
+    inversion H; subst.
+    unfolds is_indom.
+    destruct (M (R rn)); eauto; tryfalse.
+  }
+Qed.
+  
+Lemma dom_eq_setRs_stable :
+  forall vl M R,
+    dom_eq M (set_Rs R M vl).
+Proof.
+  intro vl.
+  induction vl; intros.
+  -
+    simpls; eauto.
+    eapply same_m_dom_eq; eauto.
+  -
+    destruct a.
+    simpl.
+    assert (dom_eq (set_R R M r w) (set_Rs R (set_R R M r w) vl)).
+    eauto.
+    eapply dom_eq_trans with (m2 := (set_R R M r w)); eauto.
+    eapply dom_eq_setR_stable; eauto.
+Qed.
+
+Lemma dom_eq_set_frame_stable2 :
+  forall M R rr0 rr1 rr2 rr3 rr4 rr5 rr6 rr7 fm,
+    dom_eq M (set_frame R M rr0 rr1 rr2 rr3 rr4 rr5 rr6 rr7 fm).
+Proof.
+  intros.
+  unfold set_frame.
+  destruct fm.
+  eapply dom_eq_setRs_stable; eauto.
+Qed.
+
+Lemma disjoint_setfrm_still2 :
+  forall M m R (rr0 rr1 rr2 rr3 rr4 rr5 rr6 rr7 : GenReg) fm,
+    disjoint M m ->
+    disjoint M (set_frame R m rr0 rr1 rr2 rr3 rr4 rr5 rr6 rr7 fm).
+Proof.
+  intros.
+  eapply disj_dom_eq_still; eauto.
+  eapply same_m_dom_eq; eauto.
+  eapply dom_eq_set_frame_stable2; eauto.
+Qed.
+
+Definition Fmr (R : RegFile) :=
+  R r8 :: R r9 :: R r10 :: R r11 :: R r12 :: R r13 :: R r14 :: R r15 ::
+    R r16 :: R r17 :: R r18 :: R r19 :: R r20 :: R r21 :: R r22 :: R r23 ::
+    R r24 :: R r25 :: R r26 :: R r27 :: R r28 :: R r29 :: R r30 :: R r31 :: nil.
+
+Lemma set_win_merge1 :
+  forall m1 m2 fm1 fm2 fm3 R,
+    indoms (Fmr R) m1 ->
+    disjoint m1 m2 ->
+    set_window R (merge m1 m2) fm1 fm2 fm3 = merge (set_window R m1 fm1 fm2 fm3) m2.
+Proof.
+  intros.
+  unfolds set_window.
+  rewrite fetch_some_set_frm_merge_eq; eauto.
+  rewrite fetch_some_set_frm_merge_eq; eauto.
+  rewrite fetch_some_set_frm_merge_eq; eauto.
+
+  do 2 eapply indoms_set_frm_still; eauto.
+  simpls.
+  simpljoin1.
+  repeat (split; eauto).
+
+  eapply indoms_set_frm_still.
+  simpls.
+  simpljoin1.
+  repeat (split; eauto).
+
+  simpls.
+  simpljoin1.
+  repeat (split; eauto).
+Qed.
+  
+Lemma set_win_merge2 :
+  forall m1 m2 fm1 fm2 fm3 R,
+    indoms (Fmr R) m2 ->
+    disjoint m1 m2 ->
+    set_window R (merge m1 m2) fm1 fm2 fm3 = merge m1 (set_window R m2 fm1 fm2 fm3).
+Proof.
+  intros.
+  unfolds set_window.
+  rewrite fetch_some_set_frm_merge_eq2; eauto.
+  rewrite fetch_some_set_frm_merge_eq2; eauto.
+  rewrite fetch_some_set_frm_merge_eq2; eauto.
+  do 3 try eapply disjoint_setfrm_still2; eauto.
+
+  do 2 eapply indoms_set_frm_still; eauto.
+  simpl in H.
+  simpl.
+  simpljoin1.
+  repeat (split; eauto).
+
+  eapply disjoint_setfrm_still2; eauto.
+  eapply indoms_set_frm_still; eauto.
+  simpl in H.
+  simpljoin1.
+  simpl.
+  repeat (split; eauto).
+
+  simpls.
+  simpljoin1.
+  repeat (split; eauto).
+Qed.
+
+Lemma set_window_res :
+  forall M M' R F D fm1 fm2 fm3 fm1' fm2' fm3',
+    (M, (R, F), D) |= Regs fm1 fm2 fm3 ->
+    (M', (R, F), D) |= Regs fm1' fm2' fm3' ->
+    set_window R M fm1 fm2 fm3 = M'.
+Proof.
+  intros.
+
+  >>>>>>>>>>>>>>>>>>>
   
 Lemma save_rule_sound :
   forall p q (rs rd : GenReg) v1 v2 v v' id id' F fm1 fm2 fmo fml fmi p1 oexp,
@@ -1389,13 +2841,191 @@ Proof.
   destruct_state x0.
   simpl in H9.
   simpljoin1.
+ 
+  assert (f1 = F ++ [fm1; fm2]).
+  {
+    clear - H4.
+    simpl in H4.
+    simpljoin1; eauto.
+  }
 
+  subst. 
+  lets Hf : H4.
+  eapply frame_asrt_upd with (id' := pre_cwp id) (F' := fml :: fmi :: F) in Hf; eauto.
+  simpljoin1.
+  rename x into m'.
+
+  lets Hreg : H6. 
+  eapply Regs_asrt_upd with
+  (F' := fml :: fmi :: F) (fm1' := fm1) (fm2' := fm2) (fm3' := fmo) in Hreg.
+  simpljoin1.
+  rename x into m1'. 
+  eapply asrt_FrmFree_changefrm_stable with (F' := fml :: fmi :: F) in H8; eauto.
+
+  Focus 2.
+  clear - H4 H7.
+  eapply disj_merge_disj_sep2 in H7.
+  intro.
+  simpl in H4.
+  simpljoin1.
+  unfolds regSt.
+  simpls.
+  simpljoin1.
+  unfolds disjoint.
+  specialize (H7 (r1 cwp)).
+  unfolds MemMap.set.
+  destruct_addreq_H.
+  unfolds indom; simpljoin1.
+  rewrite H in H7; tryfalse.
+  
+  assert
+    (Htt : 
+      ((merge m' (merge m1' m3)), (r1, fml :: fmi :: F), d1) |=
+      {|pre_cwp id, fml :: fmi :: F|} ** Regs fm1 fm2 fmo ** p1
+    ).
+  { 
+    eapply disj_sep_star_merge; eauto.
+    eapply disj_sep_star_merge; eauto.
+    eapply disj_dom_eq_still.
+    2 : eauto. 
+    eauto.
+    eapply same_m_dom_eq.
+    
+    eauto.
+    eapply disj_sep_merge_still; eauto.
+    eapply disj_merge_disj_sep1 in H7; eauto.
+    eapply disj_dom_eq_still; eauto.
+    eapply disj_merge_disj_sep2 in H7; eauto.
+    eapply disj_dom_eq_still; eauto.
+    eapply same_m_dom_eq; eauto.
+  }
+
+  unfolds regSt.
+  simpl in H5.
+  simpljoin1.
+  eapply H3 in Htt.
+
+  simpl in Htt.
+  simpljoin1.
+  destruct_state x.
+  destruct_state x0.
+  unfolds regSt.
+  simpl in H5, H15.
+  simpljoin1.
+  
   eexists.
   split.
+  Focus 2.
+  simpl.
+ 
+  exists (MemMap.set (r0 Rwim) (Some v) emp, (r0, fml :: fmi :: F), d0).
+  eexists.
+  split.
+
+  Focus 2.
+  split.
+  unfold regSt.
+  simpl.
+  repeat (split; eauto).
+
+  exists (MemMap.set (r0 rd) (Some (v1 +ᵢ v2)) emp, (r0, fml :: fmi :: F), d0).
+  eexists.
+  split.
+  Focus 2.
+  split; eauto.
+  unfold regSt.
+  simpl.
+  split; eauto.
+
+  simpl.
+  repeat (split; eauto).
+  eapply MemSet_same_addr_disj_stable; eauto.
+
+  simpl.
+  repeat (split; eauto).
+  clear - H1 H11 H13 H21.
+  eapply disj_dom_eq_still; eauto.
+  eapply same_m_dom_eq; eauto.
+  eapply dom_eq_merge_subst1; eauto.
+  instantiate (1 := m').
+  eapply dom_eq_sym; eauto.
+  eapply dom_eq_trans with (m2 := merge m' (merge m1' m3)).
+  eapply dom_eq_merge_still; eauto.
+  eapply same_m_dom_eq; eauto.
+  eapply dom_eq_merge_still; eauto.
+  eapply same_m_dom_eq; eauto.
+  rewrite H21.
+  eapply dom_eq_merge_still; eauto.
+  eapply dom_eq_memset_same_addr_stable; eauto.
+  eapply dom_eq_emp.
+  eapply same_m_dom_eq.
+
+  eapply SSave; eauto.
+  {  
+    clear - H4 H1 H7.
+    eapply disj_in_m2_merge_still; eauto.
+    eapply disj_in_m1_merge_still; eauto.
+    simpl in H4.
+    unfolds regSt.
+    simpls.
+    simpljoin1.
+    unfold MemMap.set.
+    destruct_addreq.
+  } 
   {
-    
+    eapply disj_in_m1_merge_still; eauto.
+    clear.
+    unfold MemMap.set.
+    destruct_addreq.
   }
-  
+  {
+    instantiate (1 := fmo).
+    clear - H1 H6 H7 H9. 
+    eapply fetch_disj_merge_still2; eauto.
+    eapply fetch_disj_merge_still2; eauto.
+    eapply fetch_disj_merge_still1; eauto.
+    eapply Regs_fetch; eauto.
+  }  
+  { 
+    eapply indom_merge_still2; eauto.
+    assert (indom (r0 rd) (merge (MemMap.set (r0 rd) (Some v') emp) m2)).
+    {
+      eapply indom_merge_still; eauto.
+      eapply memset_l_l_indom; eauto.
+    }
+    rewrite <- H21 in H15.
+    eapply indom_dom_eq_merge_subst with (m1 := m'); eauto.
+    eapply indom_dom_eq_merge_subst2 with (m2 := (merge m1' m3)); eauto.
+    eapply dom_eq_merge_still; eauto.
+    eapply dom_eq_sym; eauto.
+    eapply same_m_dom_eq; eauto.
+    eapply dom_eq_sym; eauto.
+  }
+  {
+    instantiate (1 := v1).
+    clear - H H1 Ht.
+    eapply H in Ht; eauto.
+    simpl in Ht.
+    simpljoin1.
+    eapply get_vl_merge_still2; eauto.
+  }
+  {
+    instantiate (1 := v2).
+    clear - H H1 Ht.
+    eapply H in Ht; eauto.
+    simpl in Ht.
+    simpljoin1.
+    eapply eval_opexp_merge_still2; eauto.
+  }
+  {
+    rewrite set_win_merge2; eauto.
+    rewrite set_win_merge2; eauto.
+    rewrite set_win_merge1; eauto.
+        
+    
+    >>>>>>>>>>>>>>>>>>>>>>>>>
+  }
+
 Theorem ins_rule_sound : forall p q i,
       |- {{ p }} i {{ q }} ->
       ins_sound p q i.
